@prefix rdf:        <http://www.w3.org/1999/02/22-rdf-syntax-ns#> .
@prefix rdfs:       <http://www.w3.org/2000/01/rdf-schema#> .
@prefix owl:        <http://www.w3.org/2002/07/owl#> .
@prefix xsd:        <http://www.w3.org/2001/XMLSchema#> .
@prefix skos:       <http://www.w3.org/2004/02/skos/core#> .
@prefix foaf:       <http://xmlns.com/foaf/0.1/> .
@prefix dct:        <http://purl.org/dc/terms/> .
@prefix gr:         <http://purl.org/goodrelations/v1#> .
@prefix owlTime:    <http://www.w3.org/2006/time#> .
@prefix org:        <http://www.w3.org/ns/org#> .
@prefix vcard:      <http://www.w3.org/2006/vcard/ns#> .
@prefix prov:       <http://www.w3.org/ns/prov#> .
@prefix sioc:       <http://rdfs.org/sioc/ns#> . # for follows and has_subscriber
@prefix arts:       <http://artsapi.com/def/arts/> .
@prefix keywords:   <http://artsapi.com/def/arts/keywords/> .

# Ontology metadata
#---------------------------------------------------------

arts:ontology a owl:Ontology;

    rdfs:label "Arts Organizations ontology"@en;
    rdfs:comment "Vocabulary for describing connections between organizations and agents that are members of organizations in relation to the arts sector. Includes general use classes for fine-grained classification of email correspondence."@en;

    dct:created "2014-11-20"^^xsd:date;
    dct:title "Arts Organizations ontology"@en;
    dct:contributor [foaf:mbox "alex@swirrl.com"; foaf:name "Alex Lynham"], [foaf:mbox "bill@swirrl.com"; foaf:name "Bill Roberts"];
    dct:licence <http://www.opendatacommons.org/licenses/pddl/1.0/>;
    .

# Core classes
#---------------------------------------------------------

arts:Domain a owl:Class, rdfs:Class;
    rdfs:label "A domain name or host"@en;
    rdfs:comment "A website domain name is a string that identifies an internet result such as a website. It is assumed that a domain denotes administrative authority on the part of the owner."@en;
    rdfs:isDefinedBy arts:ontology;
    .

arts:TwitterAccount a owl:Class, rdfs:Class;
    rdfs:label "A Twitter user account"@en;
    rdfs:comment "Represents a user account on the microblogging service Twitter."@en;
    rdfs:isDefinedBy arts:ontology;
    rdfs:subClassOf foaf:OnlineAccount;
    .

arts:EmailAccount a owl:Class, rdfs:Class;
    rdfs:label "An Email account. This is an abstraction that can be used to hold a mailto:URI where a foaf:Person is not available or not known, and thus cannot be used as the subject of a triple where a predicate of vcard:hasEmail or foaf:mbox points to the mailto:URI."@en;
    rdfs:comment "Represents a user email account."@en;
    rdfs:isDefinedBy arts:ontology;
    rdfs:subClassOf foaf:OnlineAccount;
    .

arts:LinkedInAccount a owl:Class, rdfs:Class;
    rdfs:label "An account on LinkedIn "@en;
    rdfs:comment "Represents a user LinkedIn account."@en;
    rdfs:isDefinedBy arts:ontology;
    rdfs:subClassOf foaf:OnlineAccount;
    .

arts:LinkedInRecommendation a owl:Class, rdfs:Class;
    rdfs:label "A recommendation created by or received by a user on the networking service LinkedIn."@en;
    rdfs:comment "Represents a written recommendation given on LinkedIn by one user to another."@en;
    rdfs:isDefinedBy arts:ontology;
    rdfs:subClassOf foaf:Document, owl:Thing;
    .

arts:LinkedInEndorsement a owl:Class, rdfs:Class;
    rdfs:label "A endorsement created by or received by a user on the networking service LinkedIn."@en;
    rdfs:comment "Once a user has posted a skill on their LinkedIn profile, other users may publicly endorse it. A LinkedIn endorsement is a document representing the connexion that takes place as a result of this activity."@en;
    rdfs:isDefinedBy arts:ontology;
    rdfs:subClassOf foaf:Document, owl:Thing;
    .

arts:LinkedInSkill a owl:Class, rdfs:Class;
    rdfs:label "A skill specified by a user on their LinkedIn profile."@en;
    rdfs:comment "A skill specified by a user on their LinkedIn profile. Once published, other users can endorse the skill publicly."@en;
    rdfs:isDefinedBy arts:ontology;
    rdfs:subClassOf foaf:Document, owl:Thing;
    .

arts:Message a owl:Class, rdfs:Class;
    rdfs:label "A Message"@en;
    rdfs:comment "Represents a message directly transmitted between two or more foaf:OnlineAccounts, appropriate subclasses or other messaging resources or identifiers. A message, unlike a Post, is directed."@en;
    rdfs:isDefinedBy arts:ontology;
    rdfs:subClassOf foaf:Document, owl:Thing;
    .

arts:Post a owl:Class, rdfs:Class;
    rdfs:label "A Post"@en;
    rdfs:comment "Represents a post; this could be a blog post or an appropriate feed update, but is distinct from a static web resource or a Message."@en;
    rdfs:isDefinedBy arts:ontology;
    rdfs:subClassOf foaf:Document, owl:Thing;
    .

arts:Tweet a owl:Class, rdfs:Class;
    rdfs:label "A Tweet"@en;
    rdfs:comment "Represents a post or Tweet on the microblogging service Twitter. This can be thought of as a Post rather than a message. Direct Messages on the service can be thought of as Messages."@en;
    rdfs:isDefinedBy arts:ontology;
    rdfs:subClassOf arts:Post;
    .

arts:Email a owl:Class, rdfs:Class;
    rdfs:label "An Email message."@en;
    rdfs:comment "An Email message."@en;
    rdfs:isDefinedBy arts:ontology;
    rdfs:subClassOf arts:Message;
    .

# Properties and relationships
#---------------------------------------------------------

arts:connection a owl:ObjectProperty, rdf:Property;
    rdfs:label "A connection"@en;
    rdfs:comment "Indicates a connection between two foaf:Person resources or two Organisations. A connection is defined as either a LinkedIn connection or two People that have exchanged one reciprocal email."@en;
    rdfs:isDefinedBy arts:ontology;
    .

arts:ownsDomain a owl:ObjectProperty, rdf:Property;
    rdfs:label "Owns domain"@en;
    rdfs:comment "Indicates a web domain that is owned by an Organization."@en;
    rdfs:isDefinedBy arts:ontology;
    rdfs:domain org:Organization;
    rdfs:range arts:Domain;
    .

arts:hasDomain a owl:ObjectProperty, rdf:Property;
    rdfs:label "Has domain"@en;
    rdfs:comment "Indicates that the thing to which this property refers has a connection to a Domain. In the case of an Email, it would refer to the Domain the Email was sent from. A foaf:OnlineAccount for example might also be linked to the Domain on which the account was registered."@en;
    rdfs:isDefinedBy arts:ontology;
    rdfs:range arts:Domain;
    .

arts:position a owl:ObjectProperty, rdf:Property;
    rdfs:label "Position"@en;
    rdfs:comment "Indicates the position or role of a foaf:Person in an organisation to which they belong."@en;
    rdfs:isDefinedBy arts:ontology;
    rdfs:domain foaf:Person;
    .

arts:department a owl:ObjectProperty, rdf:Property;
    rdfs:label "Department"@en;
    rdfs:comment "Indicates the department (in terms of an org:OrganizationalUnit) to which a foaf:Person belongs."@en;
    rdfs:isDefinedBy arts:ontology;
    rdfs:domain foaf:Person;
    rdfs:range org:OrganizationalUnit;
    .

arts:possibleDepartment a owl:ObjectProperty, rdf:Property;
    rdfs:label "Possible Department"@en;
    rdfs:comment "Indicates the department (in terms of an org:OrganizationalUnit) to which a foaf:Person has been predicated to belong, according to a heuristic algorithm internal to the ArtsAPI tool."@en;
    rdfs:isDefinedBy arts:ontology;
    rdfs:domain foaf:Person;
    rdfs:range org:OrganizationalUnit;
    .

arts:subjectArea a owl:ObjectProperty, rdf:Property;
    rdfs:label "Subject area"@en;
    rdfs:comment "Indicates an area which this foaf:Person has discussed in official correspondence above a threshold that determines they are likely to have subject area expertise or interest in this Keyword in a professional capacity within their organisation. It is a broad category that points to a resource of the KeywordCategory class and contains KeywordSubCategor(ies)."@en;
    rdfs:isDefinedBy arts:ontology;
    rdfs:domain foaf:Person;
    rdfs:range arts:KeywordCategory;
    .

arts:functionalArea a owl:ObjectProperty, rdf:Property;
    rdfs:label "Functional area"@en;
    rdfs:comment "A broad category that points to a resource of the KeywordSubCategory class. The presence of this triple means a relevant Keyword in this KeywordSubCategory must also be associated with this foaf:Person."@en;
    rdfs:isDefinedBy arts:ontology;
    rdfs:subPropertyOf arts:subjectArea;
    rdfs:domain foaf:Person;
    rdfs:range arts:KeywordSubCategory;
    .

arts:mentionedKeyword a owl:ObjectProperty, rdf:Property;
    rdfs:label "Mentioned keyword"@en;
    rdfs:comment "Indicates a Keyword that was mentioned enough times in emails by the subject (a foaf:Person) to be flagged as significant and generate this triple."@en;
    rdfs:isDefinedBy arts:ontology;
    rdfs:subPropertyOf arts:functionalArea;
    rdfs:domain foaf:Person;
    rdfs:range arts:Keyword;
    .

arts:containsKeyword a owl:ObjectProperty, rdf:Property;
    rdfs:label "Contains keyword"@en;
    rdfs:comment "Indicates a Keyword that was used in the body of this arts:Email."@en;
    rdfs:isDefinedBy arts:ontology;
    rdfs:domain arts:Email;
    rdfs:range arts:Keyword;
    .

arts:worksOn a owl:ObjectProperty, rdf:Property;
    rdfs:label "Works on"@en;
    rdfs:comment "Indicates that work is being done on a Project."@en;
    rdfs:isDefinedBy arts:ontology;
    rdfs:range foaf:Project;
    .

arts:workedOn a owl:ObjectProperty, rdf:Property;
    rdfs:label "Worked on"@en;
    rdfs:comment "Indicates that work has been done on a Project"@en;
    rdfs:isDefinedBy arts:ontology;
    rdfs:range foaf:Project;
    .

arts:linkedInProfileName a owl:ObjectProperty, rdf:Property;
    rdfs:label "LinkedIn profile name"@en;
    rdfs:comment "Indicates the name this user has given as their real name on LinkedIn."@en;
    rdfs:isDefinedBy arts:ontology;
    rdfs:domain foaf:Person;
    .

arts:hasLinkedInSkill a owl:ObjectProperty, rdf:Property;
    rdfs:label "LinkedIn Skill"@en;
    rdfs:comment "Indicates a skill that a LinkedIn user has specified on their user profile page, or a skill that has been specified in an Endorsement."@en;
    rdfs:isDefinedBy arts:ontology;
    rdfs:range arts:LinkedInSkill;
    .

arts:sender a owl:ObjectProperty, rdf:Property;
    rdfs:label "Sender"@en;
    rdfs:comment "Indicates that something (a subclass of owl:Thing) has been sent by the object of this triple. The object might be a discrete foaf:Person, Agent or mailto:URI, for example."@en;
    rdfs:isDefinedBy arts:ontology;
    .

arts:tweetSender a owl:ObjectProperty, rdf:Property;
    rdfs:label "Tweet sender"@en;
    rdfs:comment "Indicates that a Tweet was sent by the object of this triple."@en;
    rdfs:isDefinedBy arts:ontology;
    rdfs:subPropertyOf arts:sender;
    rdfs:domain arts:Tweet;
    .

arts:emailSender a owl:ObjectProperty, rdf:Property;
    rdfs:label "Email sender"@en;
    rdfs:comment "Indicates that an Email was sent by the object of this triple."@en;
    rdfs:isDefinedBy arts:ontology;
    rdfs:subPropertyOf arts:sender;
    rdfs:domain arts:Email;
    .

arts:sentAt a owl:ObjectProperty, rdf:Property;
    rdfs:label "Sent at"@en;
    rdfs:comment "A timestamp to specify when a Thing was sent."@en;
    rdfs:isDefinedBy arts:ontology;
    rdfs:range xsd:dateTime;
    .

arts:receivedAt a owl:ObjectProperty, rdf:Property;
    rdfs:label "Sent at"@en;
    rdfs:comment "A timestamp to specify when a Thing was received."@en;
    rdfs:isDefinedBy arts:ontology;
    rdfs:range xsd:dateTime;
    .

arts:subject a owl:ObjectProperty, rdf:Property;
    rdfs:label "Subject"@en;
    rdfs:comment "A string representing the main subject of a message."@en;
    rdfs:isDefinedBy arts:ontology;
    .

arts:content a owl:ObjectProperty, rdf:Property;
    rdfs:label "Content"@en;
    rdfs:comment "The content of a message."@en;
    rdfs:isDefinedBy arts:ontology;
    .

arts:emailSubject a owl:ObjectProperty, rdf:Property;
    rdfs:label "Email subject"@en;
    rdfs:comment "A string representing the subject line of a message."@en;
    rdfs:isDefinedBy arts:ontology;
    rdfs:domain arts:Email;
    rdfs:subPropertyOf arts:subject;
    .

arts:recipient a owl:ObjectProperty, rdf:Property;
    rdfs:label "Recipient"@en;
    rdfs:comment "Indicates the recipient of a message, or the intended reader, in the case of a tag or mention, where a target reader is expressed as part of metadata as opposed to directly in the messaging protocol, as with Email or Direct Messages."@en;
    rdfs:isDefinedBy arts:ontology;
    .

arts:emailRecipient a owl:ObjectProperty, rdf:Property;
    rdfs:label "Email recipient"@en;
    rdfs:comment "Indicates the recipient of an email."@en;
    rdfs:isDefinedBy arts:ontology;
    rdfs:domain arts:Email;
    rdfs:subPropertyOf arts:recipient;
    .

arts:ccRecipient a owl:ObjectProperty, rdf:Property;
    rdfs:label "CC recipient"@en;
    rdfs:comment "Indicates a email address or reference to a Person CC'd on a sent email message."@en;
    rdfs:isDefinedBy arts:ontology;
    rdfs:domain arts:Email;
    rdfs:subPropertyOf arts:recipient;
    .

arts:recommender a owl:ObjectProperty, rdf:Property;
    rdfs:label "Recommender"@en;
    rdfs:comment "Indicates the creator of a recommendation."@en;
    rdfs:isDefinedBy arts:ontology;
    rdfs:domain foaf:Person;
    rdfs:subPropertyOf arts:sender;
    .

arts:recommendee a owl:ObjectProperty, rdf:Property;
    rdfs:label "Recommendee"@en;
    rdfs:comment "Indicates the recipient of a recommendation."@en;
    rdfs:isDefinedBy arts:ontology;
    rdfs:domain foaf:Person;
    rdfs:subPropertyOf arts:recipient;
    .

arts:endorser a owl:ObjectProperty, rdf:Property;
    rdfs:label "Endorser"@en;
    rdfs:comment "Indicates the creator of an endorsement."@en;
    rdfs:isDefinedBy arts:ontology;
    rdfs:domain foaf:Person;
    rdfs:subPropertyOf arts:sender;
    .

arts:endorsee a owl:ObjectProperty, rdf:Property;
    rdfs:label "Endorsee"@en;
    rdfs:comment "Indicates the recipient of an endorsement."@en;
    rdfs:isDefinedBy arts:ontology;
    rdfs:domain foaf:Person;
    rdfs:subPropertyOf arts:recipient;
    .

arts:mentions a owl:ObjectProperty, rdf:Property;
    rdfs:label "Mentions"@en;
    rdfs:comment "Indicates a unique TwitterAccount that is mentioned in a Tweet."@en;
    rdfs:isDefinedBy arts:ontology;
    rdfs:domain arts:Tweet;
    rdfs:range arts:TwitterAccount;
    rdfs:subPropertyOf arts:recipient;
    .

# Keywords Concept Scheme and Classes - see other file
# Keywords resources - see other file

# Keywords Properties
#---------------------------------------------------------

keywords:inCategory a owl:ObjectProperty, rdf:Property;
    rdfs:label "In Category"@en;
    rdfs:comment ""@en;
    rdfs:isDefinedBy arts:ontology;
    rdfs:subPropertyOf skos:broader;
    rdfs:domain keywords:KeywordSubCategory;
    rdfs:range keywords:KeywordCategory;
    .

keywords:inSubCategory a owl:ObjectProperty, rdf:Property;
    rdfs:label "In Sub-Category"@en;
    rdfs:comment ""@en;
    rdfs:isDefinedBy arts:ontology;
    rdfs:subPropertyOf skos:broader;
    rdfs:domain keywords:Keyword;
    rdfs:range keywords:KeywordSubCategory;
    .
