@prefix rdf:        <http://www.w3.org/1999/02/22-rdf-syntax-ns#> .
@prefix rdfs:       <http://www.w3.org/2000/01/rdf-schema#> .
@prefix owl:        <http://www.w3.org/2002/07/owl#> .
@prefix xsd:        <http://www.w3.org/2001/XMLSchema#> .
@prefix skos:       <http://www.w3.org/2004/02/skos/core#> .
@prefix foaf:       <http://xmlns.com/foaf/0.1/> .
@prefix dct:        <http://purl.org/dc/terms/> .
@prefix keywords:   <http://data.artsapi.com/def/arts/keywords/> .
@prefix arts:       <http://data.artsapi.com/def/arts/> .

# Keywords Concept Scheme
#---------------------------------------------------------

keywords:keywords a skos:ConceptScheme;
    rdfs:label "ArtsAPI Keyword Hierarchy";
    dct:title "ArtsAPI Keyword Hierarchy";
    rdfs:comment "A concept scheme for keywords with nesting to represent thematic hierarchies";
    skos:hasTopConcept keywords:KeywordCategory;
    .

keywords:KeywordCategory a skos:Concept;
    rdfs:label "A category"@en;
    rdfs:comment "A category contains SubCategor(ies), which in turn contain Keywords."@en;
    skos:definition "A category contains SubCategor(ies), which in turn contain Keywords."@en;
    skos:inScheme keywords:keywords;
    .

keywords:KeywordSubCategory a skos:Concept;
    rdfs:label "A sub category"@en;
    rdfs:comment "A sub category contains Keywords."@en;
    skos:definition "A sub category contains Keywords."@en;
    skos:inScheme keywords:keywords;
    skos:broader keywords:KeywordCategory;
    .

keywords:Keyword a skos:Concept;
    rdfs:label "A Keyword"@en;
    rdfs:comment "A Keyword identified as having specific relevance to a person's role within an organisation."@en;
    skos:definition "A Keyword identified as having specific relevance to a person's role within an organisation."@en;
    skos:inScheme keywords:keywords;
    skos:broader keywords:KeywordSubCategory;
    .

# Keywords Properties
#---------------------------------------------------------

keywords:inCategory a owl:ObjectProperty, rdf:Property;
    rdfs:label "In Category"@en;
    rdfs:comment ""@en;
    rdfs:isDefinedBy arts:ontology;
    rdfs:subPropertyOf skos:broader;
    rdfs:domain keywords:KeywordSubCategory;
    rdfs:range keywords:KeywordCategory;
    .

keywords:inSubCategory a owl:ObjectProperty, rdf:Property;
    rdfs:label "In Sub-Category"@en;
    rdfs:comment ""@en;
    rdfs:isDefinedBy arts:ontology;
    rdfs:subPropertyOf skos:broader;
    rdfs:domain keywords:Keyword;
    rdfs:range keywords:KeywordSubCategory;
    .

keywords:hasInflection a owl:ObjectProperty, rdf:Property;
    rdfs:label "Has inflection"@en;
    rdfs:comment "Has an inflection of the base Keyword that can be considered equivalent for the purposes of Keyword Analysis."@en;
    rdfs:isDefinedBy arts:ontology;
    rdfs:domain keywords:Keyword;
    .